update

problemaBancnotelor.dfy
@@ -1,368 +1,497 @@
-predicate esteSolutie(sol : seq<int>, nr : int)
-   requires |sol| == 3
-   requires sol[0] >= 0
-   requires sol[1] >= 0
-   requires sol[2] >= 0
+predicate esteSolutieValida(solutie : seq<int>)
 {
-    sol[0]*1 + sol[1]*5 + sol[2]*10 == nr
+  |solutie| == 4 && solutie[0]>=0 && solutie[1]>=0 && solutie[2]>=0 && solutie[3]>=0
 }
 
-function cost(sol : seq<int>) : int 
-   requires |sol| == 3
-   requires sol[0] >= 0
-   requires sol[1] >= 0
-   requires sol[2] >= 0
+
+
+predicate esteSolutie(solutie : seq<int>, nr:int)
+  requires esteSolutieValida(solutie)
 {
-    sol[0] + sol[1] + sol[2]
+    solutie[0]*1+solutie[1]*5+solutie[2]*10+solutie[3]*20 == nr
+
 }
 
-predicate esteSolutieOptima(sol : seq<int>, nr : int)
-    requires |sol| == 3
-    requires sol[0] >= 0
-    requires sol[1] >= 0
-    requires sol[2] >= 0
+
+function cost(solutie : seq<int>):int 
+  requires esteSolutieValida(solutie)
+{
+    solutie[0]+solutie[1]+solutie[2]+solutie[3]
+}
+
+predicate esteSolutieOptima(solutie : seq<int>, nr:int)
+    requires esteSolutieValida(solutie)
 {   
-  esteSolutie(sol, nr) &&
-  forall sol' :: |sol'| == 3 && sol'[0] >= 0 && sol'[1] >=0 && sol'[2] >= 0 && esteSolutie(sol', nr) 
-          ==> cost(sol') >= cost(sol)
+  esteSolutie(solutie,nr) &&
+  forall solutieOarecare :: esteSolutieValida(solutieOarecare) && esteSolutie(solutieOarecare,nr) 
+          ==> cost(solutieOarecare) >= cost(solutie)
+
 }
 
-predicate INV(copie: int, nr: int, solutie : seq<int>)
-  requires |solutie| == 3
-  requires solutie[0] >= 0
-  requires solutie[1] >= 0
-  requires solutie[2] >= 0
+predicate INV(copie: int, nr: int, solutieFinala : seq<int>)
+  requires esteSolutieValida(solutieFinala)
 {
-   forall s1', s5', s10' :: s1'>=0 && s5'>=0 && s10'>=0 ==>
-          (esteSolutie([s1',s5',s10'],copie) ==> 
-          esteSolutie([solutie[0]+s1',solutie[1]+s5',solutie[2]+s10'],nr)) &&
-          (esteSolutieOptima([s1',s5',s10'],copie) ==> 
-          esteSolutieOptima([solutie[0]+s1',solutie[1]+s5',solutie[2]+s10'],nr))
+   forall solutieCurenta :: esteSolutieValida(solutieCurenta) ==>
+          (esteSolutie(solutieCurenta,copie) ==> 
+          esteSolutie([solutieFinala[0]+solutieCurenta[0],solutieFinala[1]+solutieCurenta[1],
+          solutieFinala[2]+solutieCurenta[2],solutieFinala[3]+solutieCurenta[3]],nr)) &&
+          (esteSolutieOptima(solutieCurenta,copie) ==> 
+          esteSolutieOptima([solutieFinala[0]+solutieCurenta[0],solutieFinala[1]+solutieCurenta[1],
+          solutieFinala[2]+solutieCurenta[2],solutieFinala[3]+solutieCurenta[3]],nr))
 }
+
 
 method gasireMaxim(nr: int) returns(s:int)
   requires nr > 0
   ensures 0 < s <= nr
-  ensures s == 1 || s == 5 || s == 10
+  ensures s == 1 || s == 5 || s == 10 || s == 20
   ensures s == 1 ==> nr < 5
   ensures s == 5 ==> 5 <= nr < 10
-  ensures s == 10 ==> nr >= 10
-  
+  ensures s == 10 ==> 10 <= nr < 20
+  ensures s == 20 ==> nr >= 20
 {
-  if(nr >= 10){
-    s := 10;
-  }
-  else
-  {
-    if(nr >= 5){
-    s := 5;
-  }
-    else{
-       if(nr < 5){
-        s := 1; 
-        }
+    if(nr >= 20)
+    {
+        s := 20;
     }
-  }
-  
+    else if(nr >= 10){
+        s := 10;
+        }
+        else if(nr >= 5){
+        s := 5;
+            }
+            else if(nr < 5){
+                s := 1; 
+            }
+
 }
 
-lemma cazMaxim1(copie: int, nr: int, solutie : seq<int>)
+
+lemma cazMaxim1(copie: int, nr: int, solutieFinala: seq<int>)
   requires copie < 5
-  requires |solutie| == 3
-  requires solutie[0] >= 0
-  requires solutie[1] >= 0
-  requires solutie[2] >= 0
-  requires INV(copie,nr,solutie)
-  ensures INV(copie-1,nr,[(solutie[0]+1),solutie[1],solutie[2]])
+  requires esteSolutieValida(solutieFinala)
+  requires INV(copie,nr,solutieFinala)
+  ensures INV(copie-1,nr,[(solutieFinala[0]+1),solutieFinala[1],solutieFinala[2],solutieFinala[3]])
 {
 
-  forall s1', s5', s10' | s1'>=0 && s5'>=0 && s10'>=0 
-          && esteSolutieOptima([s1',s5',s10'],copie-1) 
-          ensures esteSolutieOptima([solutie[0]+s1'+1,solutie[1]+s5',solutie[2]+s10'],nr)
+  forall solutieCurenta | esteSolutieValida(solutieCurenta) && esteSolutieOptima(solutieCurenta,copie-1) 
+          ensures esteSolutieOptima([solutieFinala[0]+solutieCurenta[0]+1,solutieFinala[1]+solutieCurenta[1],
+          solutieFinala[2]+solutieCurenta[2],solutieFinala[3]+solutieCurenta[3]],nr)
   {
-    assert esteSolutie([s1',s5',s10'],copie-1);
-    assert esteSolutie([s1'+1,s5',s10'],copie);
+    assert esteSolutie(solutieCurenta,copie-1);
+    assert esteSolutie([solutieCurenta[0]+1,solutieCurenta[1],solutieCurenta[2],solutieCurenta[3]],copie);
 
-    assert forall sol' :: |sol'| == 3 && sol'[0]>=0 && sol'[1]>=0 && sol'[2]>=0 
-          && esteSolutie(sol',copie-1) 
-          ==> cost(sol') >= cost([s1',s5',s10']);
-    assert esteSolutie([solutie[0]+s1'+1,solutie[1]+s5',solutie[2]+s10'],nr);
-    assert forall sol' :: |sol'| == 3 && sol'[0]>=0 && sol'[1]>=0 && sol'[2]>=0 
-          && esteSolutie(sol',nr) 
-          ==> cost(sol') >= cost([solutie[0]+s1'+1,solutie[1]+s5',solutie[2]+s10']);
+    assert forall solutieOarecare :: esteSolutieValida(solutieOarecare) && esteSolutie(solutieOarecare,copie-1) 
+          ==> cost(solutieOarecare) >= cost(solutieCurenta);
+
+    assert esteSolutie([solutieFinala[0]+solutieCurenta[0]+1,solutieFinala[1]+solutieCurenta[1],
+          solutieFinala[2]+solutieCurenta[2],solutieFinala[3]+solutieCurenta[3]],nr);
+
+    assert forall solutieOarecare :: esteSolutieValida(solutieOarecare) &&  esteSolutie(solutieOarecare,nr) 
+          ==> cost(solutieOarecare) >= cost([solutieCurenta[0]+solutieFinala[0]+1,solutieCurenta[1]+solutieFinala[1],
+          solutieCurenta[2]+solutieFinala[2],solutieCurenta[3]+solutieFinala[3]]);
   }
 
-  assert forall s1', s5', s10' :: s1'>=0 && s5'>=0 && s10'>=0 
-          && esteSolutieOptima([s1',s5',s10'],copie-1) ==> 
-          esteSolutieOptima([solutie[0]+s1'+1,solutie[1]+s5',solutie[2]+s10'],nr);
+  assert forall solutieCurenta :: esteSolutieValida(solutieCurenta) 
+          && esteSolutieOptima(solutieCurenta,copie-1) ==> 
+          esteSolutieOptima([solutieFinala[0]+solutieCurenta[0]+1,solutieFinala[1]+solutieCurenta[1],
+          solutieFinala[2]+solutieCurenta[2],solutieFinala[3]+solutieCurenta[3]],nr);
 
 }
 
-lemma cazMaxim5(copie: int,nr: int, solutie: seq<int>)
+lemma cazMaxim5(copie: int, nr: int, solutieFinala: seq<int>)
   requires 5 <= copie < 10 
-  requires |solutie| == 3
-  requires solutie[0] >= 0
-  requires solutie[1] >= 0
-  requires solutie[2] >= 0
-  requires INV(copie,nr,solutie)
-  ensures INV(copie-5,nr,[solutie[0],(solutie[1]+1),solutie[2]])
+  requires esteSolutieValida(solutieFinala)
+  requires INV(copie,nr,solutieFinala)
+  ensures INV(copie-5,nr,[solutieFinala[0],(solutieFinala[1]+1),solutieFinala[2],solutieFinala[3]])
 {
 
- forall s1', s5', s10' | s1'>=0 && s5'>=0 && s10'>=0 
-          && esteSolutieOptima([s1',s5',s10'],copie-5) 
-          ensures esteSolutieOptima([solutie[0]+s1',solutie[1]+s5'+1,solutie[2]+s10'],nr)
+ forall solutieCurenta | esteSolutieValida(solutieCurenta) && esteSolutieOptima(solutieCurenta,copie-5) 
+          ensures esteSolutieOptima([solutieFinala[0]+solutieCurenta[0],solutieFinala[1]+solutieCurenta[1]+1,
+          solutieCurenta[2]+solutieFinala[2],solutieCurenta[3]+solutieFinala[3]],nr)
   {
-    assert esteSolutie([s1',s5',s10'],copie-5);
-    assert esteSolutie([s1',s5'+1,s10'],copie);
-    assert forall sol' :: |sol'| == 3 && sol'[0]>=0 && sol'[1]>=0 && sol'[2]>=0 && esteSolutie(sol',copie-5) 
-          ==> cost(sol') >= cost([s1',s5',s10']);
-    assert esteSolutie([solutie[0]+s1',solutie[1]+s5'+1,solutie[2]+s10'],nr);
+    assert esteSolutie(solutieCurenta,copie-5);
+    assert esteSolutie([solutieCurenta[0], solutieCurenta[1]+1,solutieCurenta[2],solutieCurenta[3]],copie);
+
+    assert forall solutieOarecare :: esteSolutieValida(solutieOarecare)  && esteSolutie(solutieOarecare,copie-5) 
+          ==> cost(solutieOarecare) >= cost(solutieCurenta);
+    assert esteSolutie([solutieFinala[0]+solutieCurenta[0],solutieFinala[1]+solutieCurenta[1]+1,solutieFinala[2]+solutieCurenta[2],solutieFinala[3]+solutieCurenta[3]],nr);
     
-    assert forall sol' :: |sol'| == 3 && sol'[0]>=0 && sol'[1]>=0 && sol'[2]>=0 && esteSolutie(sol',nr)
-          ==> cost(sol') >= cost([solutie[0]+s1',solutie[1]+s5'+1,solutie[2]+s10']);
+    assert forall solutieOarecare :: esteSolutieValida(solutieOarecare) && esteSolutie(solutieOarecare,nr)
+          ==> cost(solutieOarecare) >= cost([solutieFinala[0]+solutieCurenta[0],solutieFinala[1]+solutieCurenta[1]+1,solutieFinala[2]+solutieCurenta[2],solutieFinala[3]+solutieCurenta[3]]);
   }
 
-  assert forall s1', s5', s10' :: s1'>=0 && s5'>=0 && s10'>=0 
-          && esteSolutie([s1',s5',s10'],copie-5) ==> 
-          esteSolutieOptima([solutie[0]+s1',solutie[1]+s5'+1,solutie[2]+s10'],nr);
+  assert forall solutieCurenta :: esteSolutieValida(solutieCurenta) && esteSolutie(solutieCurenta,copie-5) ==> 
+          esteSolutieOptima([solutieCurenta[0]+solutieFinala[0],solutieCurenta[1]+solutieFinala[1]+1,solutieCurenta[2]+solutieFinala[2],solutieCurenta[3]+solutieFinala[3]],nr);
 
 }
 
-lemma B(copie:int,nr: int,sol' : seq<int>, s1': int, s5' :int, s10':int)
-  requires |sol'| == 3
-  requires sol'[0]>=0
-  requires sol'[1]>=0
-  requires sol'[2]>=0
-  requires s1' >= 0
-  requires s5' >= 0
-  requires s10' >= 0
-  requires copie >=10
-  requires esteSolutie(sol',copie)
-  requires esteSolutie([s1',s5',s10'],copie-10)
-  requires esteSolutieOptima([s1',s5',s10'],copie-10)
-  ensures cost(sol') >= cost([s1',s5',(s10'+1)])
-  decreases sol'[0],sol'[1]
+lemma aux2(copie:int,solutieCurenta:seq<int>)
+  requires 10 <= copie < 20
+  requires esteSolutieValida(solutieCurenta)
+  requires esteSolutieOptima(solutieCurenta,copie-10)
+  ensures esteSolutieOptima([solutieCurenta[0], solutieCurenta[1],solutieCurenta[2]+1,solutieCurenta[3]],copie)
 {
-  assert esteSolutie(sol',copie);
-  assert esteSolutie([s1',s5',(s10'+1)],copie);
 
-  if(cost(sol') < cost([s1',s5',(s10'+1)]))
-  {
-    if(sol'[2] > (s10'+1))
+    assert esteSolutie([solutieCurenta[0], solutieCurenta[1],solutieCurenta[2]+1,solutieCurenta[3]],copie);
+    if(!esteSolutieOptima([solutieCurenta[0], solutieCurenta[1],solutieCurenta[2]+1,solutieCurenta[3]],copie))
     {
-      assert cost([sol'[0],sol'[1],(sol'[2]-1)]) < cost([s1',s5',s10']);
-      assert esteSolutieOptima([sol'[0],sol'[1],(sol'[2]-1)],(copie-10));
-      assert false;
-    }
-    else
-    {
-      if(sol'[2]<s10'+1)
+      var solopt :|esteSolutieValida(solopt) && esteSolutie(solopt,copie) && cost(solopt)<cost([solutieCurenta[0], solutieCurenta[1],solutieCurenta[2]+1,solutieCurenta[3]]);
+      assert cost([solutieCurenta[0], solutieCurenta[1],solutieCurenta[2]+1,solutieCurenta[3]]) == cost(solutieCurenta)+1;
+      assert solopt[3]==0;
+      if(solopt[2]>=1)
       {
-        assert (sol'[0]+(5*sol'[1]))>10;
+        var solopt' := [solopt[0],solopt[1],solopt[2]-1,solopt[3]];
+        assert esteSolutie(solopt',copie-10);
+        assert cost(solopt') == cost(solopt)-1;
+        assert cost(solopt)-1 < cost(solutieCurenta);
+        assert false;
+      }
+      else if(solopt[1]>=2)
+      {
+        var solopt' := [solopt[0],solopt[1]-2,solopt[2],solopt[3]];
+        assert esteSolutie(solopt',copie-10);
+        assert cost(solopt') == cost(solopt)-2;
+        assert cost(solopt)-2 < cost(solutieCurenta);
+        assert false;
+      }else if(solopt[1]>=1 && solopt[0]>=5 )
+      {
+        var solopt' := [solopt[0]-5,solopt[1]-1,solopt[2],solopt[3]];
+        assert esteSolutie(solopt',copie-10);
+        assert cost(solopt') == cost(solopt)-6;
+        assert cost(solopt)-6 < cost(solutieCurenta);
+        assert false;
+      }
+      else if(solopt[0]>=10 )
+      {
+        var solopt' := [solopt[0]-10,solopt[1],solopt[2],solopt[3]];
+        assert esteSolutie(solopt',copie-10);
+        assert cost(solopt') == cost(solopt)-10;
+        assert cost(solopt)-10 < cost(solutieCurenta);
+        assert false;
+      }
+      else{
+        assert false;
+      }
 
-        if(sol'[0]>=10)
+    }
+
+}
+
+
+
+lemma cazMaxim10(copie: int, nr: int, solutieFinala: seq<int>)
+  requires 10 <= copie < 20 
+  requires esteSolutieValida(solutieFinala) 
+  requires INV(copie,nr,solutieFinala)
+  ensures INV(copie-10,nr,[solutieFinala[0],solutieFinala[1],solutieFinala[2]+1,solutieFinala[3]])
+{
+
+ forall solutieCurenta | esteSolutieValida(solutieCurenta) && esteSolutieOptima(solutieCurenta,copie-10) 
+          ensures esteSolutieOptima([solutieFinala[0]+solutieCurenta[0],solutieFinala[1]+solutieCurenta[1],
+          solutieCurenta[2]+solutieFinala[2]+1,solutieCurenta[3]+solutieFinala[3]],nr)
+  {
+    assert esteSolutie(solutieCurenta,copie-10);
+    assert esteSolutie([solutieCurenta[0], solutieCurenta[1],solutieCurenta[2]+1,solutieCurenta[3]],copie);
+
+    aux2(copie,solutieCurenta);
+
+    assert esteSolutieOptima([solutieCurenta[0], solutieCurenta[1],solutieCurenta[2]+1,solutieCurenta[3]],copie);
+
+    assert forall solutieOarecare :: esteSolutieValida(solutieOarecare)  && esteSolutie(solutieOarecare,copie-10) 
+          ==> cost(solutieOarecare) >= cost(solutieCurenta);
+    
+
+    assert esteSolutie([solutieFinala[0]+solutieCurenta[0],solutieFinala[1]+solutieCurenta[1],1+solutieFinala[2]+solutieCurenta[2],solutieFinala[3]+solutieCurenta[3]],nr);
+
+    assert forall solutieOarecare :: esteSolutieValida(solutieOarecare) && esteSolutie(solutieOarecare,nr)
+          ==> cost(solutieOarecare) >= cost([solutieCurenta[0]+solutieFinala[0],solutieCurenta[1]+solutieFinala[1],
+                                        solutieCurenta[2]+solutieFinala[2]+1,solutieCurenta[3]+solutieFinala[3]]);
+  }
+
+  assert forall solutieCurenta :: esteSolutieValida(solutieCurenta) && esteSolutieOptima(solutieCurenta,copie-10) ==> 
+          esteSolutieOptima([solutieCurenta[0]+solutieFinala[0],solutieCurenta[1]+solutieFinala[1],
+                            solutieCurenta[2]+solutieFinala[2]+1,solutieCurenta[3]+solutieFinala[3]],nr);
+
+}
+
+
+
+lemma B(copie:int,nr: int,solutieOarecare : seq<int>, solutieCurenta: seq<int>)
+  requires esteSolutieValida(solutieOarecare)
+  requires esteSolutieValida(solutieCurenta)
+  requires copie >= 20
+  requires esteSolutie(solutieOarecare,copie)
+  requires esteSolutie(solutieCurenta,copie-20)
+  requires esteSolutieOptima(solutieCurenta,copie-20)
+  ensures cost(solutieOarecare) >= cost([solutieCurenta[0],solutieCurenta[1],solutieCurenta[2],1+solutieCurenta[3]])
+  decreases solutieOarecare[0],solutieOarecare[1],solutieOarecare[2]
+{
+  assert esteSolutie(solutieOarecare,copie);
+  assert esteSolutie([solutieCurenta[0],solutieCurenta[1],solutieCurenta[2],solutieCurenta[3]+1],copie);
+
+  if(cost(solutieOarecare) < cost([solutieCurenta[0],solutieCurenta[1],solutieCurenta[2],1+solutieCurenta[3]]))
+  {
+    if(solutieOarecare[3] > (solutieCurenta[3]+1))
+    {
+      assert cost([solutieOarecare[0],solutieOarecare[1],solutieOarecare[2],solutieOarecare[3]-1]) < cost(solutieCurenta);
+      assert esteSolutieOptima([solutieOarecare[0],solutieOarecare[1],solutieOarecare[2],solutieOarecare[3]-1],(copie-20));
+      assert false;
+      
+    }
+    else if(solutieOarecare[3] < solutieCurenta[3]+1)
+      {
+        assert (solutieOarecare[0]+(5*solutieOarecare[1])+(10*solutieOarecare[2]))>20;
+        
+        if(solutieOarecare[2]>=2)
         {
-          var sol'' := [sol'[0]-10,sol'[1],sol'[2]+1];
-          B(copie,nr,sol'', s1', s5', s10');
+            var nouaSolutieOarecare := [solutieOarecare[0],solutieOarecare[1],solutieOarecare[2]-2,solutieOarecare[3]+1];
+            B(copie,nr,nouaSolutieOarecare, solutieCurenta);
         }
-        else{
-          if(sol'[1]>=2){
-            var sol'' := [sol'[0],sol'[1]-2,sol'[2]+1];
-             B(copie,nr,sol'', s1', s5', s10');
-          }
-          else
-          {
-            var sol'' := [sol'[0]-5,sol'[1]-1,sol'[2]+1];
-             B(copie,nr,sol'', s1', s5', s10');
-          }
+        else if(solutieOarecare[2]>=1 && solutieOarecare[1]>=2)
+        {
+            var nouaSolutieOarecare := [solutieOarecare[0],solutieOarecare[1]-2,solutieOarecare[2]-1,solutieOarecare[3]+1];
+            B(copie,nr,nouaSolutieOarecare, solutieCurenta);
+        }
+        else if(solutieOarecare[2]>=1 && solutieOarecare[1]>=1 && solutieOarecare[0]>=5)
+        {
+            var nouaSolutieOarecare := [solutieOarecare[0]-5,solutieOarecare[1]-1,solutieOarecare[2]-1,solutieOarecare[3]+1];
+            B(copie,nr,nouaSolutieOarecare, solutieCurenta);
+        }
+        else if(solutieOarecare[1]>=4)
+        {
+            var nouaSolutieOarecare := [solutieOarecare[0],solutieOarecare[1]-4,solutieOarecare[2],solutieOarecare[3]+1];
+            B(copie,nr,nouaSolutieOarecare, solutieCurenta);
+        }
+        else if(solutieOarecare[1]>=3 && solutieOarecare[0]>=5)
+        {
+            var nouaSolutieOarecare := [solutieOarecare[0]-5,solutieOarecare[1]-3,solutieOarecare[2],solutieOarecare[3]+1];
+            B(copie,nr,nouaSolutieOarecare, solutieCurenta);
+        }
+        else if(solutieOarecare[1]>=2 && solutieOarecare[0]>=10)
+        {
+            var nouaSolutieOarecare := [solutieOarecare[0]-10,solutieOarecare[1]-2,solutieOarecare[2],solutieOarecare[3]+1];
+            B(copie,nr,nouaSolutieOarecare, solutieCurenta);
+        }
+        else if(solutieOarecare[1]>=1 && solutieOarecare[0]>=15)
+        {
+          var nouaSolutieOarecare := [solutieOarecare[0]-15,solutieOarecare[1]-1,solutieOarecare[2],solutieOarecare[3]+1];
+            B(copie,nr,nouaSolutieOarecare, solutieCurenta);
+        }
+        else if(solutieOarecare[0]>=20)
+        {
+            var nouaSolutieOarecare := [solutieOarecare[0]-20,solutieOarecare[1],solutieOarecare[2],solutieOarecare[3]+1];
+            B(copie,nr,nouaSolutieOarecare, solutieCurenta);
+        }
+        else if(solutieOarecare[2]>=1 && solutieOarecare[0]>=10)
+        {
+            var nouaSolutieOarecare := [solutieOarecare[0]-10,solutieOarecare[1],solutieOarecare[2]-1,solutieOarecare[3]+1];
+            B(copie,nr,nouaSolutieOarecare, solutieCurenta);
         }
       }
-    }
-    assert sol'[2] == (s10'+1);
 
-    if(sol'[1]>s5')
+    assert solutieOarecare[3] == (solutieCurenta[3]+1);
+
+    if(solutieOarecare[2]>solutieCurenta[2])
     {
-      assert cost([sol'[0],sol'[1],(sol'[2]-1)]) < cost([s1',s5',s10']);
+      assert cost([solutieOarecare[0],solutieOarecare[1],solutieOarecare[2],solutieOarecare[3]-1]) < cost(solutieCurenta);
+      assert false;
+    }
+    else if(solutieOarecare[2] < solutieCurenta[2])
+      {
+        assert (solutieOarecare[0]+(5*solutieOarecare[1]))>10;
+
+        if(solutieOarecare[0]>=10)
+        {
+          var nouaSolutieOarecare := [solutieOarecare[0]-10,solutieOarecare[1],solutieOarecare[2]+1,solutieOarecare[3]];
+          B(copie,nr,nouaSolutieOarecare, solutieCurenta);
+        }
+        else if(solutieOarecare[1]>=2){
+            var nouaSolutieOarecare := [solutieOarecare[0],solutieOarecare[1]-2,solutieOarecare[2]+1,solutieOarecare[3]];
+             B(copie,nr,nouaSolutieOarecare, solutieCurenta);
+        }
+          else
+          {
+            var nouaSolutieOarecare := [solutieOarecare[0]-5,solutieOarecare[1]-1,solutieOarecare[2]+1,solutieOarecare[3]];
+             B(copie,nr,nouaSolutieOarecare, solutieCurenta);
+          }
+        }
+        assert solutieOarecare[2] == solutieCurenta[2];
+
+      if(solutieOarecare[1]>solutieCurenta[1])
+    {
+      assert cost([solutieOarecare[0],solutieOarecare[1],solutieOarecare[2],solutieOarecare[3]-1]) < cost(solutieCurenta);
       assert false;
     }
     else
     {
-      if(sol'[1]<s5')
+      if(solutieOarecare[1]<solutieCurenta[1])
       {
-        assert sol'[0]>=5;
+        assert solutieOarecare[0]>=5;
       
-          var sol'' := [sol'[0]-5,sol'[1]+1,sol'[2]];
-          B(copie, nr, sol'', s1', s5', s10');
+          var nouaSolutieOarecare := [solutieOarecare[0]-5,solutieOarecare[1]+1,solutieOarecare[2],solutieOarecare[3]];
+          B(copie, nr, nouaSolutieOarecare, solutieCurenta);
         
       }
     }
-
-    assert sol'[1] == s5';
-
-    assert sol'[0]==s1';
-    
+    assert solutieOarecare[0]==solutieCurenta[0];
     assert false;
+
   }
 }
 
-lemma solCopie(copie:int,nr: int,sol':seq<int>, s1': int, s5' :int, s10':int)
-  requires |sol'| == 3
-  requires sol'[0]>=0
-  requires sol'[1]>=0
-  requires sol'[2]>=0
-  requires s1' >= 0
-  requires s5' >= 0
-  requires s10' >= 0
-  requires copie >=10
-  requires esteSolutie([s1',s5',s10'],copie-10)
-  requires esteSolutieOptima([s1',s5',s10'],copie-10)
-  ensures esteSolutieOptima([s1',s5',s10'+1],copie)
+lemma esteSolutiePentruCopie(copie:int,nr: int, solutieCurenta:seq<int>)
+  requires esteSolutieValida(solutieCurenta)
+  requires copie >= 20
+  requires esteSolutie(solutieCurenta,copie-20)
+  requires esteSolutieOptima(solutieCurenta,copie-20)
+  ensures esteSolutieOptima([solutieCurenta[0],solutieCurenta[1],solutieCurenta[2],1+solutieCurenta[3]],copie)
 {
-  forall sol' | |sol'| == 3 && sol'[0]>=0 && sol'[1]>=0 && sol'[2]>=0 && esteSolutie(sol',copie)
-    ensures cost(sol')>=cost([s1',s5',(s10'+1)])
+  forall solutieOarecare | esteSolutieValida(solutieOarecare) && esteSolutie(solutieOarecare,copie)
+    ensures cost(solutieOarecare)>=cost([solutieCurenta[0],solutieCurenta[1],solutieCurenta[2],1+solutieCurenta[3]])
   {
-    B(copie,nr, sol' ,s1', s5',s10');
+    B(copie,nr, solutieOarecare, solutieCurenta);
   }
   
 }
 
-lemma aux(copie: int ,nr: int, sol' : seq<int>, s1 : int, s1' : int, s5 : int, s5' : int, s10 : int, s10':int)
-  requires |sol'| == 3
-  requires sol'[0]>=0
-  requires sol'[1]>=0
-  requires sol'[2]>=0
-  requires s1 >= 0
-  requires s5 >= 0
-  requires s10 >= 0
-  requires s1' >= 0 
-  requires s5' >= 0
-  requires s10' >= 0
-  requires copie >= 10 
-  requires esteSolutieOptima([s1',s5',s10'],copie-10)
-  requires esteSolutie([s1+s1',s5+s5',s10+s10'+1],nr)
-  requires esteSolutie(sol',nr)
-  requires INV(copie,nr,[s1,s5,s10])
-  ensures cost(sol') >= cost([s1+s1',s5+s5',s10+s10'+1])
+lemma aux(copie: int ,nr: int, solutieOarecare : seq<int>, solutieFinala : seq<int>, solutieCurenta:seq<int>)
+  requires esteSolutieValida(solutieOarecare)
+  requires esteSolutieValida(solutieFinala)
+  requires esteSolutieValida(solutieCurenta)
+  requires copie >= 20
+  requires esteSolutieOptima(solutieCurenta,copie-20)
+  requires esteSolutie([solutieFinala[0]+solutieCurenta[0],solutieFinala[1]+solutieCurenta[1],solutieFinala[2]+solutieCurenta[2],1+solutieFinala[3]+solutieCurenta[3]],nr)
+  requires esteSolutie(solutieOarecare,nr)
+  requires INV(copie,nr,solutieFinala)
+  ensures cost(solutieOarecare) >= cost([solutieFinala[0]+solutieCurenta[0],solutieFinala[1]+solutieCurenta[1],solutieFinala[2]+solutieCurenta[2],1+solutieFinala[3]+solutieCurenta[3]])
 {
-  solCopie(copie,nr,sol',s1', s5', s10');
+  esteSolutiePentruCopie(copie,nr,solutieCurenta);
 }
 
-lemma cazMaxim10(copie: int,nr: int,solutie : seq<int>)
-  requires copie >= 10
-  requires |solutie| == 3
-  requires solutie[0] >= 0
-  requires solutie[1] >= 0
-  requires solutie[2] >= 0
-  requires INV(copie,nr,solutie)
-  ensures INV(copie-10,nr,[solutie[0],solutie[1],(solutie[2]+1)])
-{
-  assert forall s1', s5', s10' :: s1'>=0 && s5'>=0 && s10'>=0 ==>
-          (esteSolutie([s1',s5',s10'],copie) ==> 
-          esteSolutie([solutie[0]+s1',solutie[1]+s5',solutie[2]+s10'],nr));
 
-   forall s1', s5', s10' | s1'>=0 && s5'>=0 && s10'>=0 
-          && esteSolutie([s1',s5',s10'],copie-10) 
-          ensures esteSolutie([solutie[0]+s1',solutie[1]+s5',solutie[2]+s10'+1],nr)
+
+
+lemma cazMaxim20(copie: int,nr: int, solutieFinala : seq<int>)
+  requires copie >= 20
+  requires esteSolutieValida(solutieFinala)
+  requires INV(copie,nr,solutieFinala)
+  ensures INV(copie-20,nr,[solutieFinala[0],solutieFinala[1],solutieFinala[2],solutieFinala[3]+1])
+{
+  assert forall solutieCurenta :: esteSolutieValida(solutieCurenta) ==>
+          (esteSolutie(solutieCurenta,copie) ==> 
+          esteSolutie([solutieFinala[0]+solutieCurenta[0],solutieFinala[1]+solutieCurenta[1],solutieFinala[2]+solutieCurenta[2],solutieFinala[3]+solutieCurenta[3]],nr));
+
+   forall solutieCurenta | esteSolutieValida(solutieCurenta) 
+          && esteSolutie(solutieCurenta,copie-20) 
+          ensures esteSolutie([solutieFinala[0]+solutieCurenta[0],solutieFinala[1]+solutieCurenta[1],solutieFinala[2]+solutieCurenta[2],solutieFinala[3]+solutieCurenta[3]+1],nr)
    {
-     assert esteSolutie([s1',s5',s10'+1],copie);
+     assert esteSolutie([solutieCurenta[0],solutieCurenta[1],solutieCurenta[2],solutieCurenta[3]+1],copie);
    }
   
 
-  forall s1', s5', s10' | s1'>=0 && s5'>=0 && s10'>=0 
-          && esteSolutieOptima([s1',s5',s10'],copie-10) 
-          ensures esteSolutieOptima([solutie[0]+s1',solutie[1]+s5',solutie[2]+s10'+1],nr)
+  forall solutieCurenta | esteSolutieValida(solutieCurenta) 
+          && esteSolutieOptima(solutieCurenta,copie-20) 
+          ensures esteSolutieOptima([solutieFinala[0]+solutieCurenta[0],solutieFinala[1]+solutieCurenta[1],solutieFinala[2]+solutieCurenta[2],solutieFinala[3]+solutieCurenta[3]+1],nr)
   {
 
-    assert esteSolutie([s1',s5',s10'],copie-10);
-    assert esteSolutie([s1',s5',s10'+1],copie);
+    assert esteSolutie(solutieCurenta,copie-20);
+    assert esteSolutie([solutieCurenta[0],solutieCurenta[1],solutieCurenta[2],solutieCurenta[3]+1],copie);
 
-    assert forall sol' :: |sol'| == 3 && sol'[0]>=0 && sol'[1]>=0 && sol'[2]>=0 
-          && esteSolutie(sol',copie-10) 
-          ==> cost(sol') >= cost([s1',s5',s10']);
+    assert forall solutieOarecare :: esteSolutieValida(solutieOarecare)
+          && esteSolutie(solutieOarecare,copie-20) 
+          ==> cost(solutieOarecare) >= cost(solutieCurenta);
 
 
-    assert esteSolutie([solutie[0]+s1',solutie[1]+s5',solutie[2]+s10'+1],nr);
+    assert esteSolutie([solutieFinala[0]+solutieCurenta[0],solutieFinala[1]+solutieCurenta[1],solutieFinala[2]+solutieCurenta[2],solutieFinala[3]+solutieCurenta[3]+1],nr);
 
-    forall sol' | |sol'| == 3 && sol'[0]>=0 && sol'[1]>=0 && sol'[2]>=0 && esteSolutie(sol',nr)
-      ensures cost(sol') >= cost([solutie[0]+s1',solutie[1]+s5',solutie[2]+s10'+1])
+    forall solutieOarecare | esteSolutieValida(solutieOarecare)
+                 && esteSolutie(solutieOarecare,nr)
+      ensures cost(solutieOarecare) >= cost([solutieFinala[0]+solutieCurenta[0],solutieFinala[1]+solutieCurenta[1],solutieFinala[2]+solutieCurenta[2],1+solutieFinala[3]+solutieCurenta[3]])
       {
-          aux(copie, nr, sol', solutie[0], s1', solutie[1], s5', solutie[2], s10');
+          aux(copie, nr, solutieOarecare, solutieFinala, solutieCurenta);
       }
-   
-    assert forall sol' :: |sol'| == 3 && sol'[0]>=0 && sol'[1]>=0 && sol'[2]>=0 && esteSolutie(sol',nr) 
-          ==> cost(sol') >= cost([solutie[0]+s1',solutie[1]+s5',solutie[2]+s10'+1]);
+
+    assert forall solutieOarecare :: esteSolutieValida(solutieOarecare)
+             && esteSolutie(solutieOarecare,nr) 
+          ==> cost(solutieOarecare) >= cost([solutieFinala[0]+solutieCurenta[0],solutieFinala[1]+solutieCurenta[1],solutieFinala[2]+solutieCurenta[2],1+solutieFinala[3]+solutieCurenta[3]]);
   }
 
 
-  assert forall s1', s5', s10' :: s1'>=0 && s5'>=0 && s10'>=0 
-          && esteSolutieOptima([s1',s5',s10'],copie-10) ==> 
-          esteSolutieOptima([solutie[0]+s1',solutie[1]+s5',solutie[2]+s10'+1],nr);
+  assert forall solutieCurenta :: esteSolutieValida(solutieCurenta)
+          && esteSolutieOptima(solutieCurenta,copie-20) ==> 
+          esteSolutieOptima([solutieFinala[0]+solutieCurenta[0],solutieFinala[1]+solutieCurenta[1],solutieFinala[2]+solutieCurenta[2],1+solutieFinala[3]+solutieCurenta[3]],nr);
 
-  assert forall s1', s5', s10' :: s1'>=0 && s5'>=0 && s10'>=0 ==>
-          (esteSolutie([s1',s5',s10'],copie-10) ==> 
-          esteSolutie([solutie[0]+s1',solutie[1]+s5',solutie[2]+s10'+1],nr));
+
+  assert forall solutieCurenta :: esteSolutieValida(solutieCurenta) ==>
+          (esteSolutie(solutieCurenta,copie-20) ==> 
+          esteSolutie([solutieFinala[0]+solutieCurenta[0],solutieFinala[1]+solutieCurenta[1],solutieFinala[2]+solutieCurenta[2],1+solutieFinala[3]+solutieCurenta[3]],nr));
   
-  assert forall s1', s5', s10' :: s1'>=0 && s5'>=0 && s10'>=0 ==>        
-          (esteSolutieOptima([s1',s5',s10'],copie-10) ==> 
-          esteSolutieOptima([solutie[0]+s1',solutie[1]+s5',solutie[2]+s10'+1],nr));
+  assert forall solutieCurenta :: esteSolutieValida(solutieCurenta) ==>        
+          (esteSolutieOptima(solutieCurenta,copie-20) ==> 
+          esteSolutieOptima([solutieFinala[0]+solutieCurenta[0],solutieFinala[1]+solutieCurenta[1],solutieFinala[2]+solutieCurenta[2],solutieFinala[3]+solutieCurenta[3]+1],nr));
 
-  assert  INV(copie-10,nr,[solutie[0],solutie[1],(solutie[2]+1)]);
+  assert  INV(copie-20,nr,[solutieFinala[0],solutieFinala[1],solutieFinala[2],1+solutieFinala[3]]);
 }
 
 
-  method bancnote(nr: int) returns (sol: seq<int>)
+
+  method nrMinimBancnote(nr: int) returns (solutie: seq<int>)
     requires nr>=0
-    ensures |sol| == 3
-    ensures sol[0]>=0
-    ensures sol[1]>=0
-    ensures sol[2]>=0
-    ensures esteSolutie(sol,nr)
-    ensures esteSolutieOptima(sol,nr)
+    ensures esteSolutieValida(solutie)
+    ensures esteSolutie(solutie,nr)
+    ensures esteSolutieOptima(solutie,nr)
 {
 
-    var copie :=  nr;
+    var copie:=  nr;
     var s1 := 0;
     var s5 := 0;
     var s10 := 0;
+    var s20 := 0;
     while(copie > 0)
       decreases copie
       invariant 0<=copie<=nr
-      invariant esteSolutie([s1,s5,s10],nr-copie)
-      invariant INV(copie,nr,[s1,s5,s10])
+      invariant esteSolutie([s1,s5,s10,s20],nr-copie)
+      invariant INV(copie,nr,[s1,s5,s10,s20])
     {
         var i := 0;
         var s := gasireMaxim(copie);
         if( s == 1){
-            cazMaxim1(copie,nr,[s1,s5,s10]);
+            cazMaxim1(copie,nr,[s1,s5,s10,s20]);
             s1:=s1+1;
-            assert esteSolutie([s1,s5,s10],nr-(copie-1));
-            assert INV(copie-1,nr,[s1,s5,s10]);
+            assert esteSolutie([s1,s5,s10,s20],nr-(copie-1));
+            assert INV(copie-1,nr,[s1,s5,s10,s20]);
         }
-        else{
-            if(s == 5)
+        else if(s == 5)
             {
-                cazMaxim5(copie,nr,[s1,s5,s10]);
+                cazMaxim5(copie,nr,[s1,s5,s10,s20]);
                 s5:=s5+1;
-                assert esteSolutie([s1,s5,s10],nr-(copie-5));
-                assert INV(copie-5,nr,[s1,s5,s10]);
+                assert esteSolutie([s1,s5,s10,s20],nr-(copie-5));
+                assert INV(copie-5,nr,[s1,s5,s10,s20]);
+
+            }
+            else if (s == 10){
+                cazMaxim10(copie,nr,[s1,s5,s10,s20]);
+                s10:=s10+1;
+                assert esteSolutie([s1,s5,s10,s20],nr-(copie-10));
+                assert INV(copie-10,nr,[s1,s5,s10,s20]);
 
             }
             else{
-                cazMaxim10(copie,nr,[s1,s5,s10]);
-                s10:=s10+1;
-                assert esteSolutie([s1,s5,s10],nr-(copie-10));
-                assert INV(copie-10,nr,[s1,s5,s10]);
-
+                cazMaxim20(copie,nr,[s1,s5,s10,s20]);
+                s20:=s20+1;
+                assert esteSolutie([s1,s5,s10,s20],nr-(copie-20));
+                assert INV(copie-20,nr,[s1,s5,s10,s20]);
             }
-        }
+
         copie := copie-s;
     }
-    sol := [s1,s5,s10];
+    solutie := [s1,s5,s10,s20];
 }
 
 
 method Main() {
-  var nr:= 38;
-  var sol:=bancnote(nr);
+  var nr:= 58;
+  var sol:=nrMinimBancnote(nr);
   print sol;
 }
